
# A-Level Further Core 1
## Sum and Product
- If $\alpha$ and $\beta$ are roots of the equation $ax^2 + bx + c = 0$, then:
    - $\alpha + \beta = -\frac{b}{a}$
    - $\alpha\beta = \frac{c}{a}$
- If $\alpha$, $\beta$ and $\gamma$ are roots of the equation $ax^3 + bx^2 + cx + d = 0$, then:
    - $\alpha + \beta + \gamma = \Sigma\alpha = -\frac{b}{a}$
    - $\alpha\beta + \beta\gamma + \gamma\alpha = \Sigma\alpha\beta = \frac{c}{a}$
    - $\alpha\beta\gamma = -\frac{d}{a}$
- If $\alpha$, $\beta$, $\gamma$ and $\delta$ are roots of the equation $ax^4 + bx^3 + cx^2 + dx + e = 0$, then:
    - $\alpha + \beta + \gamma + \delta = \Sigma\alpha = -\frac{b}{a}$
    - $\alpha\beta + \alpha\gamma + \alpha\delta + \beta\gamma + \beta\delta + \gamma\delta = \Sigma\alpha\beta = \frac{c}{a}$
    - $\alpha\beta\gamma + \alpha\beta\delta + \alpha\gamma\delta + \beta\gamma\delta = \Sigma\alpha\beta\gamma = -\frac{d}{a}$
    - $\alpha\beta\gamma\delta = \frac{e}{a}$
> [!NOTE] How to remember
> A good way to remember is that the sum of increasing amount of roots is equal to the next coefficient over $a$ with alternating sign:
> - For Individual: $-\frac{b}{a}$
> - For Pairs: $\frac{c}{a}$
> - For Triplets: $-\frac{d}{a}$
> - For Quadruplets: $\frac{e}{a}$
>*(it goes $b, c, d, e$ and $-, +, -, +$)*
## Other Rules
- The rules for reciprocals:
    - Quadratic: $\frac{1}{\alpha} + \frac{1}{\beta} = \frac{\alpha + \beta}{\alpha\beta}$
    - Cubic: $\frac{1}{\alpha} + \frac{1}{\beta} + \frac{1}{\gamma} = \frac{\alpha\beta + \beta\gamma + \gamma\alpha}{\alpha\beta\gamma}$
    - Quartic: $\frac{1}{\alpha} + \frac{1}{\beta} + \frac{1}{\gamma} + \frac{1}{\delta} = \frac{\alpha\beta\gamma + \beta\gamma\delta + \gamma\delta\alpha + \delta\alpha\beta}{\alpha\beta\gamma\delta}$
- The rules for products of powers:
    - Quadratic: $\alpha^n \times \beta^n = (\alpha\beta)^n$
    - Cubic: $\alpha^n \times \beta^n \times \gamma^n = (\alpha\beta\gamma)^n$
    - Quartic: $\alpha^n \times \beta^n \times \gamma^n \times \delta^n = (\alpha\beta\gamma\delta)^n$
- The rules for sums of squares:
    - Quadratic: $\alpha^2 + \beta^2 = (\alpha + \beta)^2 - 2\alpha\beta$
    - Cubic: $\alpha^2 + \beta^2 + \gamma^2 = (\alpha + \beta + \gamma)^2 - 2(\alpha\beta + \beta\gamma + \gamma\alpha)$
    - Quartic: $\alpha^2 + \beta^2 + \gamma^2 + \delta^2 = (\alpha + \beta + \gamma + \delta)^2 - 2(\alpha\beta + \alpha\gamma + \alpha\delta + \beta\gamma + \beta\delta + \gamma\delta)$
- The rules for sums of cubes:
    - Quadratic: $\alpha^3 + \beta^3 = (\alpha + \beta)^3 - 3\alpha\beta(\alpha + \beta)$
    - Cubic: $\alpha^3 + \beta^3 + \gamma^3 = (\alpha + \beta + \gamma)^3 - 3(\alpha + \beta + \gamma)(\alpha\beta + \beta\gamma + \gamma\alpha) + 3\alpha\beta\gamma$


# Flashcards
#Maths/A-Level-Further-Core/Sum-Product-Of-Roots/Main, #Maths/Topics/Roots

What are the sum and product formulas for roots $\alpha$ and $\beta$ of a quadratic equation $ax^2 + bx + c = 0$?
?
- $\alpha + \beta = -\frac{b}{a}$
- $\alpha\beta = \frac{c}{a}$ 

What are the sum and product formulas for roots $\alpha$, $\beta$, and $\gamma$ of a cubic equation $ax^3 + bx^2 + cx + d = 0$?
?
- $\alpha + \beta + \gamma = \Sigma\alpha = -\frac{b}{a}$
- $\alpha\beta + \beta\gamma + \gamma\alpha = \Sigma\alpha\beta = \frac{c}{a}$
- $\alpha\beta\gamma = -\frac{d}{a}$ 

What are the sum and product formulas for roots $\alpha$, $\beta$, $\gamma$, and $\delta$ of a quartic equation $ax^4 + bx^3 + cx^2 + dx + e = 0$?
?
- $\alpha + \beta + \gamma + \delta = \Sigma\alpha = -\frac{b}{a}$
- $\alpha\beta + \alpha\gamma + \alpha\delta + \beta\gamma + \beta\delta + \gamma\delta = \Sigma\alpha\beta = \frac{c}{a}$
- $\alpha\beta\gamma + \alpha\beta\delta + \alpha\gamma\delta + \beta\gamma\delta = \Sigma\alpha\beta\gamma = -\frac{d}{a}$
- $\alpha\beta\gamma\delta = \frac{e}{a}$ 

#Maths/A-Level-Further-Core/Sum-Product-Of-Roots/Other-Rules, #Maths/Topics/Roots

What is the rule for reciprocals of roots in a quadratic equation?
?
$\frac{1}{\alpha} + \frac{1}{\beta} = \frac{\alpha + \beta}{\alpha\beta}$ 

What is the rule for reciprocals of roots in a cubic equation?
?
$\frac{1}{\alpha} + \frac{1}{\beta} + \frac{1}{\gamma} = \frac{\alpha\beta + \beta\gamma + \gamma\alpha}{\alpha\beta\gamma}$ 

What is the rule for reciprocals of roots in a quartic equation?
?
$\frac{1}{\alpha} + \frac{1}{\beta} + \frac{1}{\gamma} + \frac{1}{\delta} = \frac{\alpha\beta\gamma + \beta\gamma\delta + \gamma\delta\alpha + \delta\alpha\beta}{\alpha\beta\gamma\delta}$ 

What is the rule for sums of squares of roots in a quadratic equation?
?
$\alpha^2 + \beta^2 = (\alpha + \beta)^2 - 2\alpha\beta$ 

What is the rule for sums of squares of roots in a cubic equation?
?
$\alpha^2 + \beta^2 + \gamma^2 = (\alpha + \beta + \gamma)^2 - 2(\alpha\beta + \beta\gamma + \gamma\alpha)$ 

What is the rule for sums of squares of roots in a quartic equation?
?
$\alpha^2 + \beta^2 + \gamma^2 + \delta^2 = (\alpha + \beta + \gamma + \delta)^2 - 2(\alpha\beta + \alpha\gamma + \alpha\delta + \beta\gamma + \beta\delta + \gamma\delta)$ 

What is the rule for sums of cubes of roots in a quadratic equation?
?
$\alpha^3 + \beta^3 = (\alpha + \beta)^3 - 3\alpha\beta(\alpha + \beta)$ 

What is the rule for sums of cubes of roots in a cubic equation?
?
$\alpha^3 + \beta^3 + \gamma^3 = (\alpha + \beta + \gamma)^3 - 3(\alpha + \beta + \gamma)(\alpha\beta + \beta\gamma + \gamma\alpha) + 3\alpha\beta\gamma$ 