# A-Level Further Core 1
## Sum and Product of Roots
### Quadratic $ax^2 + bx + c = 0$
$\alpha + \beta = -\frac{b}{a}$
$\alpha\beta = \frac{c}{a}$
### Cubic $ax^3 + bx^2 + cx + d = 0$
$\alpha + \beta + \gamma = \Sigma\alpha = -\frac{b}{a}$
$\alpha\beta\gamma = -\frac{d}{a}$
### Quartic $ax^4 + bx^3 + cx^2 + dx + e = 0$
$\alpha + \beta + \gamma + \delta = \Sigma\alpha = -\frac{b}{a}$
$\alpha\beta + \alpha\gamma + \alpha\delta + \beta\gamma + \beta\delta + \gamma\delta = \Sigma\alpha\beta = \frac{c}{a}$
$\alpha\beta\gamma + \alpha\beta\delta + \alpha\gamma\delta + \beta\gamma\delta = \Sigma\alpha\beta\gamma = -\frac{d}{a}$
$\alpha\beta\gamma\delta = \frac{e}{a}$
### How to remember
A good way to remember is that the sum of increasing amount of roots is equal to the next coefficient over $a$ with alternating sign *(it goes $b, c, d, e$ and $-, +, -, +$)*:
 - For Individual: $-\frac{b}{a}$
 - For Pairs: $\frac{c}{a}$
 - For Triplets: $-\frac{d}{a}$
 - For Quadruplets: $\frac{e}{a}$
## Reciprocals of Roots
Quadratic: $\displaystyle \frac{1}{\alpha} + \frac{1}{\beta} = \frac{\alpha + \beta}{\alpha\beta}$
Cubic: $\displaystyle \frac{1}{\alpha} + \frac{1}{\beta} + \frac{1}{\gamma} = \frac{\alpha\beta + \beta\gamma + \gamma\alpha}{\alpha\beta\gamma}$
Quartic: $\displaystyle \frac{1}{\alpha} + \frac{1}{\beta} + \frac{1}{\gamma} + \frac{1}{\delta} = \frac{\alpha\beta\gamma + \beta\gamma\delta + \gamma\delta\alpha + \delta\alpha\beta}{\alpha\beta\gamma\delta}$
## Sum of squares
Quadratic: $\alpha^2 + \beta^2 = (\alpha + \beta)^2 - 2\alpha\beta$
Cubic: $\alpha^2 + \beta^2 + \gamma^2 = (\alpha + \beta + \gamma)^2 - 2(\alpha\beta + \beta\gamma + \gamma\alpha)$
Quartic: $\alpha^2 + \beta^2 + \gamma^2 + \delta^2 = (\alpha + \beta + \gamma + \delta)^2 - 2(\alpha\beta + \alpha\gamma + \alpha\delta + \beta\gamma + \beta\delta + \gamma\delta)$
## Sum of cubes
Quadratic: $\alpha^3 + \beta^3 = (\alpha + \beta)^3 - 3\alpha\beta(\alpha + \beta)$
Cubic: $\alpha^3 + \beta^3 + \gamma^3 = (\alpha + \beta + \gamma)^3 - 3(\alpha + \beta + \gamma)(\alpha\beta + \beta\gamma + \gamma\alpha) + 3\alpha\beta\gamma$

## Linear Transformations of Roots
Given a polynomial in terms of $x$ with roots $\alpha, \beta, \gamma$, you can find the polynomial in terms of $w$ with roots $(k\alpha + c)$, $(k\beta + c)$, $(k\gamma + c)$ by using the equation $w = kx + c$, then rearranging for $x$ and plugging into the original polynomial and expanding and simplifying.

---
# Flashcards
## A-Level Further Core 1
#z_Legacy/Maths/A-Levels/Further-Core/Roots-of-Polynomials, #Maths/Topics/Roots

What are the sum and product formulas for roots of polynomials?
?
$\Sigma\alpha = -\frac{b}{a}\quad\Sigma\alpha\beta = \frac{c}{a} \quad\Sigma\alpha\beta\gamma = -\frac{d}{a} \quad\alpha\beta\gamma\delta = \frac{e}{a}$     

What is the rule for sums of squares of roots in a quadratic equation?
?
$\alpha^2 + \beta^2 = (\alpha + \beta)^2 - 2\alpha\beta$ 

What is the rule for sums of squares of roots in a cubic equation?
?
$\alpha^2 + \beta^2 + \gamma^2 = (\alpha + \beta + \gamma)^2 - 2(\alpha\beta + \beta\gamma + \gamma\alpha)$   

What is the rule for sums of squares of roots in a quartic equation?
?
$\alpha^2 + \beta^2 + \gamma^2 + \delta^2 = (\alpha + \beta + \gamma + \delta)^2 - 2(\alpha\beta + \alpha\gamma + \alpha\delta + \beta\gamma + \beta\delta + \gamma\delta)$  

What is the rule for sums of cubes of roots in a quadratic equation?
?
$\alpha^3 + \beta^3 = (\alpha + \beta)^3 - 3\alpha\beta(\alpha + \beta)$    

What is the rule for sums of cubes of roots in a cubic equation?
?
$\alpha^3 + \beta^3 + \gamma^3 = (\alpha + \beta + \gamma)^3 - 3(\alpha + \beta + \gamma)(\alpha\beta + \beta\gamma + \gamma\alpha) + 3\alpha\beta\gamma$   

Given a polynomial in terms of $x$ with roots $\alpha, \beta, \gamma$, How can find the polynomial in terms of $w$ with roots $(k\alpha + c)$, $(k\beta + c)$, $(k\gamma + c)$?
?
By using the equation $w = kx + c$, then rearranging for $x$ and plugging into the original polynomial and expanding and simplifying.    